Boogie examples now in a loop

Examples/Boogie/samSmokeTest1.bpl
@@ -2,13 +2,31 @@ var i: int;
 
 procedure Main() returns ()
 	modifies i;
-	ensures i==200;
-{	
+{
+	var counter: int;
+	
 	Initialize: 
 		i := 0;
-		goto Node1;
-		
-	Node1:
+		counter := 0;
+		goto LoopHead,End;
+	
+	LoopHead:
+		assume counter < 5;
+		call Loop ();
+		assert i == 200;
+		counter := counter + 1;
+		goto LoopHead,End;
+	
+	End:
+		assume counter == 5;
+		return;
+}
+
+procedure Loop() returns ()
+	modifies i;
+	ensures i == 200;
+{
+	Node1Block:
 		i := 200;
 		return;
 }
