Examples/Boogie/samSmokeTest2.bpl
@@ -2,6 +2,28 @@ var i: int;
 
 procedure Main() returns ()
 	modifies i;
+{
+	var counter: int;
+	
+	Initialize: 
+		i := 0;
+		counter := 0;
+		goto LoopHead,End;
+	
+	LoopHead:
+		assume counter < 5;
+		call Loop ();
+		assert i == 200;
+		counter := counter + 1;
+		goto LoopHead,End;
+	
+	End:
+		assume counter == 5;
+		return;
+}
+
+procedure Loop() returns ()
+	modifies i;
 	ensures i==200;
 {	
 	Initialize: 
